testing/Complexnr/README.md
@@ -1,3 +1,3 @@
 # complexnr
 
-Lampe proofs for the [complexnr](https://github.com/manu-bhadoria/complexnr) Noir library.
+Lampe proofs for the [complexnr](https://github.com/manu-bhadoria/complexnr) Noir library (commit [`0557831`](https://github.com/manu-bhadoria/complexnr/tree/055783156928dcd949e3b9f61d1b596f55794bc5)).
